\begin{gather}
  \pd_{\text{pool}}(\boldsymbol{\phi}) = 
    \prod_{\modelindex = 1}^{\Nm}
    \pd_{\text{pool}}(\phi_{\modelindex}),
  \quad  \text{where for } \modelindex' = 1 \text{ or } \Nm, \text{ and } \modelindex = 2, \ldots, \Nm - 1 \\
  \pd_{\text{pool}}(\phi_{\modelindex'}) =
    g^{\modelindex'}(\pd_{\modelindex'}(\phi_{\modelindex' \cap \modelindex' + 1}), \pd_{\modelindex' + 1}(\phi_{\modelindex' \cap \modelindex' + 1})),\\
  \pd_{\text{pool}}(\phi_{\modelindex}) =
    g^{\modelindex}(\pd_{\modelindex - 1}(\phi_{\modelindex - 1 \cap \modelindex}), \pd_{\modelindex}(\phi_{\modelindex - 1 \cap \modelindex}, \phi_{\modelindex \cap \modelindex + 1}), \pd_{\modelindex + 1}(\phi_{\modelindex \cap \modelindex + 1}))
  \label{eqn:bad-alterative-one}
\end{gather}