\begin{gather}
  \pd_{2}(\phi_{1 \cap 2}) \pd_{\text{meld}}^{12}(\phi_{2 \cap 3}) =
  \pd_{\text{meld}}^{23}(\phi_{1 \cap 2}) \pd_{2}(\phi_{2 \cap 3}) = 
  \pd_{2}(\phi_{1 \cap 2}, \phi_{2 \cap 3}) 
  \label{eqn:coinciding-equalities-one}
  \\[1ex]
  \pd_{\text{pool}}^{12}(\phi_{1 \cap 2}) \pd_{\text{pool}}^{(12)3}(\phi_{2 \cap 3}) =
  \pd_{\text{pool}}^{1(23)}(\phi_{1 \cap 2}) \pd_{\text{pool}}^{23}(\phi_{2 \cap 3}) = 
  \pd_{\text{pool}}(\phi_{1 \cap 2}, \phi_{2 \cap 3}).
  \label{eqn:coinciding-equalities-two}
\end{gather}