\begin{align}
  \int_{0}^{t} h_{i}(u)\text{d}u &=
    \int_{0}^{t} 
      \lambda u ^{\lambda - 1} 
      \exp\{
        \beta_{0, i, k} + \beta_{1, i, k} u
      \} 
    \text{d}u \\
  &=
    \lambda
    \exp\{\beta_{0, i, k}\}
    \frac{\Gamma(\lambda)}{-\beta_{1, i, k}^{\lambda}}
    \int_{0}^{t}
      \frac{-\beta_{1, i, k}^{\lambda}}{\Gamma(\lambda)}
      u^{\lambda - 1}
      \exp\{\beta_{1, i, k} u\}
    \text{d}u \\
  &= 
    \lambda
    \exp\{\beta_{0, i, k}\}
    \frac{\Gamma(\lambda)}{-\beta_{1, i, k}^{\lambda}}
    \frac{1}{\Gamma(\lambda)}
    \gamma(\lambda, -\beta_{1, i k}t)
  \label{eqn:submodel-two-hazard-integral}
\end{align}