\begin{align}
  \pd_{\text{pool, lin}}(\phi) &=
    \frac{1}{K_{\text{lin}}(\lambda)}
    \sum_{\modelindex = 1}^{\Nm} \lambda_{\modelindex} \pd_{\modelindex}(\phi), \quad
  K_{\text{lin}}(\lambda) = \int \sum_{\modelindex = 1}^{\Nm} \lambda_{\modelindex} \pd_{\modelindex}(\phi) \text{d}\phi, \label{eqn:orig-pooling-linear}\\
  \pd_{\text{pool, log}}(\phi) &=  
    \frac{1}{K_{\text{log}}(\lambda)}
    \prod_{\modelindex = 1}^{\Nm} \pd_{\modelindex}(\phi)^{\lambda_{\modelindex}}, \quad
  K_{\text{log}}(\lambda) = \int \prod_{\modelindex = 1}^{\Nm} \pd_{\modelindex}(\phi)^{\lambda_{\modelindex}} \text{d}\phi,
  \label{eqn:orig-pooling-logarithmic}
\end{align}