\begin{equation}
\begin{gathered}
  \pd_{\text{pool}} (\phi_{1 \cap 2}, \phi_{2 \cap 3}) =
  g_{\text{log}}(\phi_{1 \cap 2}, \phi_{2 \cap 3}) =
  \frac{1}{K_{\text{log}}(\lambda)}
  \pd_{1}(\phi_{1 \cap 2})^{\lambda_{1}} 
  \pd_{2}(\phi_{1 \cap 2}, \phi_{2 \cap 3})^{\lambda_{2}}
  \pd_{3}(\phi_{2 \cap 3})^{\lambda_{3}}, \\
  K_{\text{log}}(\lambda) = 
  \int
    \pd_{1}(\phi_{1 \cap 2})^{\lambda_{1}} 
    \pd_{2}(\phi_{1 \cap 2}, \phi_{2 \cap 3})^{\lambda_{2}}
    \pd_{3}(\phi_{2 \cap 3})^{\lambda_{3}}
  \text{d}\phi_{1 \cap 2}, \phi_{2 \cap 3}
  \label{eqn:pooled-prior-overall}
\end{gathered}
\end{equation}