\begin{equation}
\begin{gathered}
  \pd_{\text{pool}} (\phi_{1 \cap 2}, \phi_{2 \cap 3}) = 
  g_{\text{lin}}(\phi_{1 \cap 2}, \phi_{2 \cap 3}) =
  \frac{1}{K_{\text{lin}}(\lambda)}
  \pd_{\text{pool}, 1}(\phi_{1 \cap 2}) 
  \pd_{\text{pool}, 2}(\phi_{2 \cap 3}), \\
  K_{\text{lin}}(\lambda) = 
    \int 
      \pd_{\text{pool}, 1}(\phi_{1 \cap 2}) 
      \pd_{\text{pool}, 2}(\phi_{2 \cap 3})
    \text{d}\phi_{1 \cap 2}, \phi_{2 \cap 3}.
  \label{eqn:silly-linear-overall}
\end{gathered}
\end{equation}