\begin{align}
  \pd_{\text{pool, dict}} (\boldsymbol{\phi}) =
    g_{\text{dict}}(\pd_{1}(\phi_{1 \cap 2}), \pd_{2}(\phi_{1 \cap 2}, \phi_{2 \cap 3}), \pd_{3}(\phi_{2 \cap 3})) &=
    \pd_{1}(\phi_{1 \cap 2}) \pd_{3}(\phi_{2 \cap 3}) \label{eqn:dictatorial-pooling-one} \\
  \pd_{\text{pool, dict}} (\boldsymbol{\phi}) =
    g_{\text{dict}}(\pd_{1}(\phi_{1 \cap 2}), \pd_{2}(\phi_{1 \cap 2}, \phi_{2 \cap 3}), \pd_{3}(\phi_{2 \cap 3})) &=
    \pd_{2}(\phi_{1 \cap 2}, \phi_{2 \cap 3}), \label{eqn:dictatorial-pooling-two}
\end{align}